theory/x64Disassembler.thy
@@ -3,6 +3,7 @@ imports
   Main
   rBPFCommType
   x64Syntax
+  x64Assembler
 begin
 
 (*
@@ -42,30 +43,283 @@ else None)"
 
 definition x64_decode :: "nat \<Rightarrow> x64_bin \<Rightarrow> (nat * instruction) option" where
 "x64_decode pc l_bin = (
+if pc \<ge> length l_bin then None else 
   let h = l_bin!pc in
-    if h = 0xc3 then Some (1, Pret)
+  if h = 0xc3 then Some (1, Pret)
+  else if unsigned_bitfield_extract_u8 4 4 h \<noteq> 0b0100 then  \<comment> \<open> h is not rex  \<close>
+      \<comment> \<open> R1 [opcode] \<close>
+      \<comment> \<open> P2885 `PUSH: qwordregister (alternate encoding)`   -> ` 0100 W00BS : 0101 0 reg64` \<close>
+      if unsigned_bitfield_extract_u8 3 5 h = 0b01010 then
+        let reg2 = unsigned_bitfield_extract_u8 0 3 h in
+        let dst  = bitfield_insert_u8 3 1 reg2 0 in
+        case ireg_of_u8 dst of None \<Rightarrow> None | Some dst \<Rightarrow> (
+          Some (1, Ppushl_r dst))
+      \<comment> \<open> P2885 `POP: qwordregister (alternate encoding)`   -> ` 0100 W00B : 0101 1 reg64 ` \<close>
+      else if unsigned_bitfield_extract_u8 3 5 h = 0b01011 then
+        let reg2 = unsigned_bitfield_extract_u8 0 3 h in
+        let dst  = bitfield_insert_u8 3 1 reg2 0 in
+        case ireg_of_u8 dst of None \<Rightarrow> None | Some dst \<Rightarrow> (
+          Some (1, Ppopl dst))
+      else None
   else 
-  let w = unsigned_bitfield_extract_u8 3 1 h in
-  let r = unsigned_bitfield_extract_u8 2 1 h in
-  let x = unsigned_bitfield_extract_u8 1 1 h in
-  let b = unsigned_bitfield_extract_u8 0 1 h in
-  let op = l_bin!(pc+1) in 
-  let reg = l_bin!(pc+2) in 
-  let modrm = unsigned_bitfield_extract_u8 6 2 reg in
-  let reg1  = unsigned_bitfield_extract_u8 3 3 reg in
-  let reg2  = unsigned_bitfield_extract_u8 0 3 reg in
-  let src   = bitfield_insert_u8 3 1 reg1 r in
-  let dst   = bitfield_insert_u8 3 1 reg2 b in
-  if op = 0x01 then if modrm = 0b11 then
+    let w = unsigned_bitfield_extract_u8 3 1 h in
+    let r = unsigned_bitfield_extract_u8 2 1 h in
+    let x = unsigned_bitfield_extract_u8 1 1 h in
+    let b = unsigned_bitfield_extract_u8 0 1 h in
+    let op = l_bin!(pc+1) in
+    if unsigned_bitfield_extract_u8 3 5 op = 0b01010 then
+        let reg2 = unsigned_bitfield_extract_u8 0 3 op in
+        let dst  = bitfield_insert_u8 3 1 reg2 b in
+        case ireg_of_u8 dst of None \<Rightarrow> None | Some dst \<Rightarrow> (
+          if w = 0 \<and> r = 0 \<and> x = 0 then
+            Some (2, Ppushl_r dst)
+          else None)
+      \<comment> \<open> P2885 `POP: qwordregister (alternate encoding)`   -> ` 0100 W00B : 0101 1 reg64 ` \<close>
+    else if unsigned_bitfield_extract_u8 3 5 op = 0b01011 then
+        let reg2 = unsigned_bitfield_extract_u8 0 3 op in
+        let dst  = bitfield_insert_u8 3 1 reg2 b in
+        case ireg_of_u8 dst of None \<Rightarrow> None | Some dst \<Rightarrow> (
+          if w = 0 \<and> r = 0 \<and> x = 0 then
+            Some (2, Ppopl dst)
+          else None)
+    else
+      let w = unsigned_bitfield_extract_u8 3 1 h in
+      let r = unsigned_bitfield_extract_u8 2 1 h in
+      let x = unsigned_bitfield_extract_u8 1 1 h in
+      let b = unsigned_bitfield_extract_u8 0 1 h in
+      let op = l_bin!(pc+1) in
+      let reg = l_bin!(pc+2) in 
+      let modrm = unsigned_bitfield_extract_u8 6 2 reg in
+      let reg1  = unsigned_bitfield_extract_u8 3 3 reg in
+      let reg2  = unsigned_bitfield_extract_u8 0 3 reg in
+      let src   = bitfield_insert_u8 3 1 reg1 r in
+      let dst   = bitfield_insert_u8 3 1 reg2 b in
+      if op = 0x01 then 
+           if modrm = 0b11 then
               case ireg_of_u8 src of None \<Rightarrow> None | Some src \<Rightarrow> (
               case ireg_of_u8 dst of None \<Rightarrow> None | Some dst \<Rightarrow> (
                 if w = 1 \<and> x = 0 then 
-                  Some (3, Paddq_rr dst src)
+                  Some (3, Paddq_rr dst src) \<comment> \<open> 0b01001000\<close>
                 else None))
-  else None
-else None)"
+              else None
+      else if op = 0xf7 then 
+           if modrm = 0b11 \<and> reg1 = 0b100 then 
+              case ireg_of_u8 dst of None \<Rightarrow> None | Some dst \<Rightarrow> (
+              if w = 1 \<and> r = 0 \<and> x = 0 then 
+                Some (3, Pmulq_r dst) 
+              else None)
+           else None
+      else if op = 0x89 then
+            if modrm = 0b11 then 
+            \<comment> \<open> P2882 `MOV register1 to register2` -> `0100 WR0B : 1000 100w : 11 reg1 reg2` \<close>
+            \<comment> \<open> P2882 `MOV qwordregister1 to qwordregister2` -> `0100 1R0B : 1000 1001 : 11 reg1 reg2` \<close>
+              case ireg_of_u8 src of None \<Rightarrow> None | Some src \<Rightarrow> (
+              case ireg_of_u8 dst of None \<Rightarrow> None | Some dst \<Rightarrow> (
+                if w = 1 \<and> x = 0 then   \<comment> \<open> rex should be `W=1` and `X=0`\<close> 
+                  Some (3, Pmovq_rr dst src) 
+                else None)) 
+            else None
+      else None)"
 
-value "x64_decode 0 [[0b01001000,0b00000001,0b11011000],[]]"
+
+value "x64_decode 0 [0b01001000,0b00000001,0b11011000,0xc3]"
+
+
+(*
+fun x64_decodes_aux ::  "nat \<Rightarrow> x64_bin list \<Rightarrow> (nat * instruction) option list " where
+"x64_decodes_aux _ [] = [None]" |
+"x64_decodes_aux pc (h#t) = (if pc \<le> length (h#t) then let ins' = x64_decode pc h in 
+                              (case ins' of None \<Rightarrow> [None] |
+                                 Some (len, v) \<Rightarrow> [Some (len, v) ] @ x64_decodes_aux pc t)
+                            else [None])"
+
+fun x64_decodes_aux ::  "nat \<Rightarrow> x64_bin list \<Rightarrow> (nat * instruction) option list " where
+"x64_decodes_aux _ [] = [None]" |
+"x64_decodes_aux pc (h#t) = (if pc \<le> length (h#t) then let ins' = x64_decode pc h in 
+                              (case ins' of None \<Rightarrow> [None] |
+                                 Some (len, v) \<Rightarrow> [Some (len, v) ] @ x64_decodes_aux pc t)
+                            else [None])"
+*)
+
+(*
+fun x64_decodes_aux ::  "nat \<Rightarrow> x64_bin \<Rightarrow> (nat * instruction) option list " where
+"x64_decodes_aux _ [] = [None]" |
+"x64_decodes_aux pc xs = (if pc \<ge> length xs then [None] 
+                          else let xs' = drop pc xs; ins' = x64_decode 0 xs' in 
+                              (case ins' of None \<Rightarrow> [None] |
+                                 Some (len, v) \<Rightarrow> [Some (len, v)] @ x64_decodes_aux (len-1) (drop 1 xs')))"
+
+definition x64_decodes:: "nat \<Rightarrow> x64_bin \<Rightarrow> (nat * instruction) list option" where
+"x64_decodes pc xs = (let x = x64_decodes_aux pc xs in if x = [None] then None  
+                   else Some (map Option.the (butlast x)))
+
+*)
+
+(*fun x64_decodes_aux ::  "nat \<Rightarrow> nat \<Rightarrow> x64_bin \<Rightarrow> (nat * instruction) option list " where
+"x64_decodes_aux 0 _ _ = []" |
+"x64_decodes_aux (Suc num) pc xs = (if pc \<ge> length xs then [] else 
+                                      let ins' = x64_decode pc xs in 
+                              (case ins' of None \<Rightarrow> [None] |
+                                 Some (len, v) \<Rightarrow> [Some (len, v)] @ x64_decodes_aux num (pc+len) xs))"
+
+definition x64_decodes:: "nat \<Rightarrow> nat \<Rightarrow> x64_bin \<Rightarrow> (nat * instruction) list option" where
+"x64_decodes num pc xs = (let x = x64_decodes_aux num pc xs in if x = [None] then None  
+                   else Some (map Option.the x))"
+
+*)
+
+
+(*fun x64_decodes_aux ::  "nat \<Rightarrow> nat \<Rightarrow> x64_bin \<Rightarrow> (nat * instruction) list option" where
+"x64_decodes_aux 0 _ _ = Some []" |
+"x64_decodes_aux (Suc num) pc xs = (if pc \<ge> length xs then None else 
+                                      let ins' = x64_decode pc xs in (case ins' of 
+                                        None \<Rightarrow> None |
+                                        Some (len, v) \<Rightarrow>  
+                                          (case x64_decodes_aux num (pc+len) xs of
+                                            None \<Rightarrow> None |
+                                            Some res \<Rightarrow> Some ((len, v)#res))))"*)
+
+
+fun x64_decodes_aux ::  "nat \<Rightarrow> nat \<Rightarrow> x64_bin \<Rightarrow> (nat * instruction) list option" where
+"x64_decodes_aux 0 _ _ = Some []" |
+"x64_decodes_aux (Suc num) pc xs = ( let ins' = x64_decode pc xs in (case ins' of 
+                                        None \<Rightarrow> None |
+                                        Some (len, v) \<Rightarrow>  
+                                          (case x64_decodes_aux num pc (drop len xs) of
+                                            None \<Rightarrow> None |
+                                            Some res \<Rightarrow> Some ((len, v)#res))))"
+
+(*lemma x64_decodes_aux_induct:"x64_decodes_aux (n+m) pc xs = Some res \<Longrightarrow>
+  x64_decodes_aux n pc xs = Some res1 \<Longrightarrow>
+  pc' = pc + sum_list (map fst res1) \<Longrightarrow>
+  x64_decodes_aux m pc' xs = Some res2 \<Longrightarrow>
+  res = res1@res2"
+  apply(induction n arbitrary: m pc xs res res1 pc' res2)
+   apply simp
+  subgoal for n m pc xs res res1 pc' res2
+    apply simp
+    apply(split if_splits, simp_all)
+    apply(cases "x64_decode pc xs",simp_all)
+    subgoal for a apply(cases a,simp_all)
+      subgoal for aa b apply(cases "x64_decodes_aux n (pc + aa) xs",simp_all)
+        subgoal for ab apply(cases "x64_decodes_aux (n + m) (pc + aa) xs",simp_all)
+          subgoal for ac 
+            by (smt (verit, best) append_Cons fst_conv group_cancel.add1 list.simps(9) sum_list.Cons)
+          done
+        done
+      done
+    done
+  done*)
+
+lemma x64_decodes_aux_equiv:
+  "Some res = x64_decode pc ins \<Longrightarrow>
+  Some resn = x64_decodes_aux 1 pc ins \<Longrightarrow>
+  [res] = resn"
+  apply(cases "x64_decode pc ins",simp_all)
+  (*apply(split if_splits,simp_all)*)
+  done
+
+lemma x64_decodes_aux_induct_aux1:"
+  x64_decodes_aux (Suc n) pc xs = Some res \<Longrightarrow>
+  x64_decode pc xs = Some res1 \<Longrightarrow>
+  len = (fst res1) \<Longrightarrow>
+  x64_decodes_aux n pc (drop len xs) = Some res2 \<Longrightarrow>
+  res = res1#res2"
+  apply(induction n arbitrary: pc xs res res1 len res2)
+   apply simp
+  subgoal for n pc xs res res1 len res2 
+    by (metis (mono_tags, lifting) old.prod.case option.inject option.simps(5) prod.collapse x64_decodes_aux.simps(2))
+  done
+
+lemma x64_decodes_aux_induct_aux2:
+  "x64_decodes_aux (Suc n) pc xs = Some res \<Longrightarrow> 
+  x64_decode pc xs = Some res1 \<Longrightarrow>
+  len = (fst res1) \<Longrightarrow>
+  x64_decodes_aux n pc (drop len xs) \<noteq> None"
+  apply(cases "x64_decodes_aux n pc (drop len xs)",simp_all)
+  apply(cases "res1",simp_all)
+  done
+
+lemma x64_decodes_aux_induct2:
+  assumes a0:"x64_decodes_aux (Suc n) pc xs = Some res" and
+  a1:"x64_decode pc xs = Some res1" and
+  a2:"len = (fst res1)" 
+shows "\<exists> res2. x64_decodes_aux n pc (drop len xs) = Some res2 \<and> res = res1#res2"
+  using x64_decodes_aux_induct_aux2 a0 a1 a2 x64_decodes_aux_induct_aux1 by fast
+
+value "x64_decodes_aux 2 0 [0xc3,0xc2,0b01001000,0b00000001,0b11011000]"
+
+value "x64_decodes_aux 2 0 [0xc3,0b01001000,0b00000001,0b11011000]"
+
+value "x64_decodes_aux 1 1 [0xc3,0b01001000,0b00000001,0b11011000]"
+
+value "x64_decodes_aux 0 1 [0xc3,0b01001000,0b00000001,0b11011000]"
+
+value "x64_decodes_aux 5 1 [0xc3,0b01001000,0b00000001,0b11011000]"
+
+
+
+(*lemma "x64_decodes_aux (Suc n) pc xs = Some res \<Longrightarrow>
+  x64_decode pc xs = Some res1 \<Longrightarrow>
+  len = (fst res1) \<Longrightarrow>
+  \<exists> res2. x64_decodes_aux n pc (drop len xs) = Some res2 \<and> res = res1#res2"
+  using x64_decodes_aux_induct2 
+apply(split if_splits, simp_all)
+    done*)
+
+
+(*lemma x64_decodes_aux_induct2:"
+  x64_decodes_aux (Suc n) pc xs = Some res \<Longrightarrow>
+  x64_decode pc xs = Some res1 \<Longrightarrow>
+  pc' = pc + (fst res1) \<Longrightarrow>
+  x64_decodes_aux n pc' xs = Some res2 \<Longrightarrow>
+  res = res1#res2"
+  sorry*)
+
+(*
+lemma x64_decodes_aux_induct2:"
+  x64_decodes_aux (Suc n) pc xs = Some res \<Longrightarrow>
+  x64_decode pc xs = Some res1 \<Longrightarrow>
+  pc' = pc + (fst res1) \<Longrightarrow>
+  x64_decodes_aux n pc' xs = Some res2 \<Longrightarrow>
+  res = res1#res2"
+  apply(induction n arbitrary: pc xs res res1 pc' res2)
+   apply simp
+  subgoal for pc xs res res1 pc' res2
+    apply(split if_splits, simp_all)
+    done
+  subgoal for n pc xs res res1 pc' res2 
+
+lemma
+  "x64_decode pc xs = Some res1 \<Longrightarrow> 
+  x64_decodes_aux 1 pc xs = Some res2  \<Longrightarrow>
+  [res1] = res2"
+
+
+(*x64_decodes_aux (Suc n) pc xs = Some res \<Longrightarrow> *)
+lemma x64_decodes_aux_induct3:"
+  x64_decode pc xs = Some res1 \<Longrightarrow>
+  len = (fst res1) \<Longrightarrow>
+  x64_decodes_aux n (pc+len) xs = Some res2 \<Longrightarrow>
+  x64_decodes_aux n pc (drop len xs) = Some res3 \<Longrightarrow> 
+  res2 = res3"
+  sorry
+
+
+lemma hhh:"a = take len xs \<Longrightarrow> b = drop len xs \<Longrightarrow> a@b = xs"
+  by simp
+
+lemma hhhh:"take (length xs) xs = xs"
+  by simp
+
+lemma "x64_decodes_aux (Suc n) 0 xs = Some res \<Longrightarrow>
+  x64_decodes 0 (take len xs) = Some res1 \<Longrightarrow>
+  len = fst res1 \<Longrightarrow>
+  x64_decodes_aux n 0 (drop len xs) = Some res2 \<Longrightarrow>
+  res = res1#res2"
+  sorry
+*)
+
 
 end
 
