theory/x64Semantics.thy
@@ -3,7 +3,7 @@ section \<open> x64 Semantics \<close>
 theory x64Semantics
 imports
   Main
-  rBPFCommType Val Mem x64Syntax x64Disassembler
+  rBPFCommType Val Mem x64Syntax x64Disassembler x64Assembler
 begin
 
 (*axiomatization x64_decode :: "nat \<Rightarrow> u8 list \<Rightarrow> (nat * instruction) option"*)
@@ -37,13 +37,58 @@ definition exec_ret :: "memory_chunk \<Rightarrow> mem \<Rightarrow> regset \<Ri
       _ \<Rightarrow> Stuck)
 )"
 
+definition exec_pop :: "usize \<Rightarrow> u64 \<Rightarrow> memory_chunk \<Rightarrow> mem \<Rightarrow> regset \<Rightarrow> ireg \<Rightarrow> outcome" where
+"exec_pop pc sz chunk m rs rd = (
+  let nsp = (rs SP) + (u64_of_memory_chunk chunk) in
+    let addr = (rs SP) in
+      case Mem.loadv chunk m addr of
+        None \<Rightarrow> Stuck |
+        Some (Vlong v) => let rs1 = rs#rd <- v in
+          Next (pc + sz) (rs1# SP <- nsp) m
+)"
+
+definition exec_push :: "usize \<Rightarrow> u64 \<Rightarrow> memory_chunk \<Rightarrow> mem \<Rightarrow> regset \<Rightarrow> usize \<Rightarrow> outcome" where
+"exec_push pc sz chunk m rs v = ( 
+  let nsp = (rs SP) - (u64_of_memory_chunk chunk) in
+      case Mem.storev chunk m nsp (Vlong v) of
+        None \<Rightarrow> Stuck |
+        Some m' => Next (pc + sz) (rs#SP <- nsp) m'
+)"
+
 definition exec_instr :: "instruction \<Rightarrow> u64 \<Rightarrow> u64 \<Rightarrow> regset \<Rightarrow> mem \<Rightarrow> outcome" where
 "exec_instr i sz pc rs m = (\<comment> \<open> sz is the binary size (n-byte) of current instruction  \<close>
   case i of
   Paddq_rr  rd r1 \<Rightarrow> Next (pc + sz) (rs#rd <- ((rs rd) + (rs r1))) m |
   Pret            \<Rightarrow> exec_ret M64 m rs |
-  _               \<Rightarrow> Stuck
+  Ppopl     rd    \<Rightarrow> exec_pop pc sz M32 m rs rd |
+  Ppushl_r  r1    \<Rightarrow> exec_push pc sz M32 m rs (rs r1) |
+  Pmovq_rr rd r1  \<Rightarrow> Next (pc + sz) (rs#rd <- (rs r1)) m |
+  Pmulq_r   r1    \<Rightarrow> let rs1 = rs#RAX <- ((rs RAX)*(rs r1)) in
+                     Next (pc + sz) (rs1# RDX <-( (rs RAX)*(rs r1) div (2 ^ 32))) m 
 )"
+(*
+definition exec_instr :: "instruction \<Rightarrow> u64 \<Rightarrow> regset \<Rightarrow> mem \<Rightarrow> outcome" where
+"exec_instr i pc rs m = (\<comment> \<open> sz is the binary size (n-byte) of current instruction  \<close>
+  case i of
+  Paddq_rr  rd r1 \<Rightarrow> Next (pc + 3) (rs#rd <- ((rs rd) + (rs r1))) m |
+  Pret            \<Rightarrow> exec_ret M64 m rs |
+  Ppopl     rd    \<Rightarrow> exec_pop pc 2 M32 m rs rd |
+  Ppushl_r  r1    \<Rightarrow> exec_push pc 2 M32 m rs (rs r1) |
+  Pmovq_rr rd r1  \<Rightarrow> Next (pc + 3) (rs#rd <- (rs r1)) m |
+  Pmulq_r   r1    \<Rightarrow> let rs1 = rs#RAX <- ((rs RAX)*(rs r1)) in
+                     Next (pc + 3) (rs1# RDX <-( (rs RAX)*(rs r1) div (2 ^ 32))) m 
+)"
+*)
+(*
+  Pmovq_rr src R11
+
+  Ppushl_r RDX
+
+  RAX=RAX*R11
+  RDX=RAX*R11 div 2^32
+
+  Ppopl RDX
+*)
 
 (*fun x64_sem :: "nat \<Rightarrow> x64_bin \<Rightarrow> outcome \<Rightarrow> outcome" where
 "x64_sem 0 _ st = st" |
@@ -67,10 +112,10 @@ fun x64_sem :: "nat \<Rightarrow> x64_bin \<Rightarrow> outcome \<Rightarrow> ou
 )"
 
 fun x64_sem1 :: "nat \<Rightarrow> u64 \<Rightarrow> (nat \<times> u64 \<times> x64_bin) list \<Rightarrow> outcome \<Rightarrow> outcome" where
-"x64_sem1 0 _ _ st = (let st_temp = (
-  case st of
+"x64_sem1 0 _ _ st = (let xst_temp =
+   case st of
     Next xpc rs m \<Rightarrow> Next 0 rs m |
-    Stuck \<Rightarrow> Stuck) in st_temp)" |
+    Stuck \<Rightarrow> Stuck in xst_temp )" |
 "x64_sem1 (Suc n) pc lt xst = (
   let (num,off,l) = lt!(unat pc) in
   let xst_temp = (
@@ -80,7 +125,72 @@ fun x64_sem1 :: "nat \<Rightarrow> u64 \<Rightarrow> (nat \<times> u64 \<times> 
   let xst' = x64_sem num l xst_temp in (
     x64_sem1 n (pc+off) lt xst'))"
 
+(*
+definition init_reg_map :: "regset" where
+"init_reg_map = (\<lambda> _. 0) (RAX:= 0b00000011, RBX:= 0b00000001)"
 
+definition init_map::"mem" where
+"init_map = Map.empty"
+
+value "init_reg_map RBX"
+
+value "init_reg_map RCX"
+
+value "init_mem 0"
+
+value "x64_sem 2 [0b01001000,0b00000001,0b11011000,0b11000011] (Next (0::u64) (init_reg_map) m)"
+value "x64_sem 1 [0b01001000,0b00000001,0b11011000,0b11000011] (Next (0::u64) (init_reg_map) m)"
+value "x64_sem 0 [0b01001000,0b00000001,0b11011000,0b11000011] (Next (0::u64) (init_reg_map) m)"
+
+value "x64_sem 1 [0b11000011] (Next (0::u64) (init_reg_map) m)"
+
+value "x64_sem 2 [0b11000011] (Next (0::u64) (init_reg_map) m)"
+
+value "x64_sem1 (2::nat) 1 [((1::nat),(1::u64),[0b01001000,0b00000001,0b11011000]),((1::nat),(1::u64),[0b11000011])] (Next (0::u64) (init_reg_map) m)"
+
+lemma "x64_sem1 (1::nat) 1 [((1::nat),(1::u64),[0b01001000,0b00000001,0b11011000]),((1::nat),(1::u64),[0b11000011])] (Next xpc rs m)  = exec_instr Pret 1 0 rs m "
+  using x64_decode_def by simp*)
+
+fun interp3 :: "instruction list \<Rightarrow> outcome \<Rightarrow> outcome" where
+"interp3 [] s = s" |
+"interp3 (ins#l) st = (
+  case st of
+  Stuck \<Rightarrow> Stuck |
+  Next pc rs m \<Rightarrow> 
+    interp3 l (exec_instr ins 1 pc rs m)
+)"
+
+(*
+fun interp3 :: "instruction list \<Rightarrow> outcome \<Rightarrow> outcome" where
+"interp3 [] s = s" |
+"interp3 (ins#l) st = (
+  case st of
+  Stuck \<Rightarrow> Stuck |
+  Next pc rs m \<Rightarrow> (
+    let x = (x64_encode ins) in
+      case x of None \<Rightarrow> Stuck |
+                Some res \<Rightarrow> 
+          let result = x64_decode 0 res in
+              case result of None \<Rightarrow> Stuck |
+                             Some res \<Rightarrow> let len = fst res
+    in interp3 l (exec_instr ins (of_nat len) pc rs m)
+))"
+
+
+
+fun interp3 :: "instruction list \<Rightarrow> outcome \<Rightarrow> outcome" where
+"interp3 [] s = s" |
+"interp3 (ins#l) st = (
+  case st of
+  Stuck \<Rightarrow> Stuck |
+  Next pc rs m \<Rightarrow> (
+    let len = (case ins of Pret \<Rightarrow> 1 |
+                  Ppopl dst \<Rightarrow> 2 |
+                  Ppushl_r dst \<Rightarrow> 2 |
+                   _ \<Rightarrow> 3 )
+    in interp3 l (exec_instr ins len pc rs m)
+))"
+*)
 value "x64_sem1 0 "
 
 (*definition x64_sem1 ::"nat \<Rightarrow> (nat \<times> x64_bin) list \<Rightarrow> outcome \<Rightarrow> outcome" where
@@ -108,30 +218,6 @@ fun interp3 :: "instruction list \<Rightarrow> outcome \<Rightarrow> outcome" wh
 ))"
 *)
 
-definition init_reg_map :: "regset" where
-"init_reg_map = (\<lambda> _. 0) (RAX:= 0b00000011, RBX:= 0b00000001)"
-
-definition init_map::"mem" where
-"init_map = Map.empty"
-
-value "init_reg_map RBX"
-
-value "init_reg_map RCX"
-
-value "init_mem 0"
-
-value "x64_sem 2 [0b01001000,0b00000001,0b11011000,0b11000011] (Next (0::u64) (init_reg_map) m)"
-value "x64_sem 1 [0b01001000,0b00000001,0b11011000,0b11000011] (Next (0::u64) (init_reg_map) m)"
-value "x64_sem 0 [0b01001000,0b00000001,0b11011000,0b11000011] (Next (0::u64) (init_reg_map) m)"
-
-value "x64_sem 1 [0b11000011] (Next (0::u64) (init_reg_map) m)"
-
-value "x64_sem 2 [0b11000011] (Next (0::u64) (init_reg_map) m)"
-
-value "x64_sem1 (2::nat) 1 [((1::nat),(1::u64),[0b01001000,0b00000001,0b11011000]),((1::nat),(1::u64),[0b11000011])] (Next (0::u64) (init_reg_map) m)"
-
-lemma "x64_sem1 (1::nat) 1 [((1::nat),(1::u64),[0b01001000,0b00000001,0b11011000]),((1::nat),(1::u64),[0b11000011])] (Next xpc rs m)  = exec_instr Pret 1 0 rs m "
-  using x64_decode_def by simp
 
 type_synonym x64_state = outcome
 
