theory/Proof1.thy
@@ -6,16 +6,56 @@ imports
 begin
 
 value "x64_decode 0 (the (x64_encode (Paddq_rr RAX RBX)))"
-           
+
 lemma x64_encode_decode_consistency:
-  "Some l_bin = x64_encode ins \<Longrightarrow>
+ "Some l_bin = x64_encode ins \<Longrightarrow>
     x64_decode 0 l_bin = Some (length l_bin, ins)"
+ 
   apply(cases ins,simp_all)
-   prefer 2 apply(unfold x64_decode_def, simp_all)
   subgoal for dst src 
-        apply (unfold Let_def construct_rex_to_u8_def construct_modsib_to_u8_def)
+    \<comment> \<open> Paddq_rr \<close> 
+    apply (unfold Let_def construct_rex_to_u8_def construct_modsib_to_u8_def)
     subgoal by (cases src; simp;cases dst; auto simp add: x64_decode_def bitfield_insert_u8_def Let_def ireg_of_u8_def
           Suc3_eq_add_3 add.commute)
     done
+   apply(unfold x64_decode_def;auto)
+  subgoal for dst
+    apply (unfold Let_def construct_rex_to_u8_def construct_modsib_to_u8_def)
+ subgoal by (cases dst; auto simp add: x64_decode_def bitfield_insert_u8_def Let_def ireg_of_u8_def)
   done
+  defer
+ subgoal for dst src
+  \<comment> \<open> Pmovq_rr \<close> 
+   apply (unfold Let_def construct_rex_to_u8_def construct_modsib_to_u8_def)
+   (*apply(erule conjE; erule conjE)*)
+   subgoal by (cases src; cases dst; auto simp add: x64_decode_def bitfield_insert_u8_def Let_def ireg_of_u8_def)
+    done
+  subgoal for dst 
+    \<comment> \<open> Pmulq_r \<close> 
+    apply (unfold Let_def construct_rex_to_u8_def construct_modsib_to_u8_def)
+    subgoal by (cases dst; auto simp add: x64_decode_def bitfield_insert_u8_def Let_def ireg_of_u8_def)
+    done
+  subgoal for dst
+    \<comment> \<open> Ppopl_i \<close> 
+    apply (unfold Let_def construct_rex_to_u8_def construct_modsib_to_u8_def)
+    apply (cases dst; auto simp add: x64_decode_def bitfield_insert_u8_def Let_def ireg_of_u8_def)
+  done
+  done
+
+(*lemma x64_encodes_decodes_consistency:
+  "Some l_bin = x64_encodes2 ins \<Longrightarrow>
+    x64_decodes 0 l_bin = Some ins_list \<Longrightarrow>
+    map snd ins_list = ins" 
+  sorry*)
+(*
+value "x64_decode 0 [0b01001000,0b00000001,0b11011000]"
+value "x64_decodes_aux 0 [0xc3,0b01001000,0b00000001,0b11011000]"
+value "x64_decodes 0 [0xc3,0b01001000,0b00000001,0b11011000]"
+value "x64_decode 1 [0xc3,0b01001000,0b00000001,0b11011000]"
+value "x64_encodes_suffix []"
+value "x64_decodes 0 []"*)
+
+
+
+
 end
